pftstep => PFConfiguration.step

src/drf/APF.v
@@ -27,147 +27,151 @@ Require Import Race.
 
 Set Implicit Arguments.
 
-Inductive pftstep: forall (e:MachineEvent.t) (tid:Ident.t) (c1 c2: Configuration.t), Prop :=
-| pftstep_intro
-    e tid c1 lang st1 lc1 e2 st3 lc3 sc3 memory3
-    (TID: IdentMap.find tid c1.(Configuration.threads) = Some (existT _ lang st1, lc1))
-    (STEPS: rtc (tau (@AThread.program_step _)) (Thread.mk _ st1 lc1 c1.(Configuration.sc) c1.(Configuration.memory)) e2)
-    (STEP: AThread.program_step e e2 (Thread.mk _ st3 lc3 sc3 memory3)):
-    pftstep (ThreadEvent.get_machine_event e) tid c1 (Configuration.mk (IdentMap.add tid (existT _ _ st3, lc3) c1.(Configuration.threads)) sc3 memory3)
-.
-Hint Constructors pftstep.
+Module APFConfiguration.
 
-Definition pftstep_all (c0 c1: Configuration.t) :=
-  union (fun e => union (pftstep e)) c0 c1.
-Hint Unfold pftstep_all.
+  Inductive step: forall (e:MachineEvent.t) (tid:Ident.t) (c1 c2: Configuration.t), Prop :=
+  | step_intro
+      e tid c1 lang st1 lc1 e2 st3 lc3 sc3 memory3
+      (TID: IdentMap.find tid c1.(Configuration.threads) = Some (existT _ lang st1, lc1))
+      (STEPS: rtc (tau (@AThread.program_step _)) (Thread.mk _ st1 lc1 c1.(Configuration.sc) c1.(Configuration.memory)) e2)
+      (STEP: AThread.program_step e e2 (Thread.mk _ st3 lc3 sc3 memory3)):
+      step (ThreadEvent.get_machine_event e) tid c1 (Configuration.mk (IdentMap.add tid (existT _ _ st3, lc3) c1.(Configuration.threads)) sc3 memory3)
+  .
+  Hint Constructors step.
 
-Inductive opt_pftstep: forall (e: MachineEvent.t) (tid: Ident.t) (c1 c2: Configuration.t), Prop :=
-| pftstep_none
-    tid c:
-    opt_pftstep MachineEvent.silent tid c c
-| pftstep_some
-    e tid c1 c2
-    (STEP: pftstep e tid c1 c2):
-    opt_pftstep e tid c1 c2
-.
-Hint Constructors opt_pftstep.
+  Definition step_all (c0 c1: Configuration.t) :=
+    union (fun e => union (step e)) c0 c1.
+  Hint Unfold step_all.
 
-Definition pf_racefree (c1:Configuration.t): Prop :=
-  forall c2
-         (STEPS: rtc pftstep_all c1 c2)
-         (RACE: pf_race c2), False.
-
-Lemma pf_racefree_step c1 c2 e tid
-      (RACEFREE : pf_racefree c1)
-      (STEP : pftstep e tid c1 c2) :
-  pf_racefree c2.
-Proof.
-  ii. eapply RACEFREE.
-  - econs 2; eauto.
-  - auto.
-Qed.
-
-Lemma pftstep_future
+  Inductive opt_step: forall (e: MachineEvent.t) (tid: Ident.t) (c1 c2: Configuration.t), Prop :=
+  | step_none
+      tid c:
+      opt_step MachineEvent.silent tid c c
+  | step_some
       e tid c1 c2
-      (STEP: pftstep e tid c1 c2)
-      (WF1: Configuration.wf c1):
-  Configuration.wf c2.
-Proof.
-  inv WF1. inv WF. inv STEP; s.
-  exploit THREADS; ss; eauto. i.
-  exploit AThread.rtc_tau_step_future.
-  { eapply rtc_implies; try apply STEPS. eapply tau_mon.
-    i. econs. econs 2; eauto. } all: eauto. s. i. des.
-  exploit AThread.step_future.
-  { econs 2; eauto. } all: eauto. s. i. des.
-  econs; ss. econs.
-  i. Configuration.simplify.
-  - exploit THREADS; try apply TH1; eauto. i. des.
-    exploit AThread.rtc_tau_step_disjoint.
+      (STEP: step e tid c1 c2):
+      opt_step e tid c1 c2
+  .
+  Hint Constructors opt_step.
+
+  Definition pf_racefree (c1:Configuration.t): Prop :=
+    forall c2
+           (STEPS: rtc step_all c1 c2)
+           (RACE: pf_race c2), False.
+
+  Lemma pf_racefree_step c1 c2 e tid
+        (RACEFREE : pf_racefree c1)
+        (STEP : step e tid c1 c2) :
+    pf_racefree c2.
+  Proof.
+    ii. eapply RACEFREE.
+    - econs 2; eauto.
+    - auto.
+  Qed.
+
+  Lemma step_future
+        e tid c1 c2
+        (STEP: step e tid c1 c2)
+        (WF1: Configuration.wf c1):
+    Configuration.wf c2.
+  Proof.
+    inv WF1. inv WF. inv STEP; s.
+    exploit THREADS; ss; eauto. i.
+    exploit AThread.rtc_tau_step_future.
     { eapply rtc_implies; try apply STEPS. eapply tau_mon.
-      i. econs. econs 2; eauto. } all: eauto. i. des.
-    exploit AThread.step_disjoint.
-    { econs 2; eauto. } all: eauto. i. des. ss.
-    symmetry. auto.
-  - exploit THREADS; try apply TH2; eauto. i. des.
-    exploit AThread.rtc_tau_step_disjoint.
-    { eapply rtc_implies; try apply STEPS. eapply tau_mon.
-      i. econs. econs 2; eauto. } all: eauto. i. des.
-    exploit AThread.step_disjoint.
-    { econs 2; eauto. } all: eauto. i. des. ss.
-  - eapply DISJOINT; [|eauto|eauto]. auto.
-  - i. Configuration.simplify.
-    exploit THREADS; try apply TH; eauto. i.
-    exploit AThread.rtc_tau_step_disjoint.
-    { eapply rtc_implies; try apply STEPS. eapply tau_mon.
-      i. econs. econs 2; eauto. } all: eauto. i. des.
-    exploit AThread.step_disjoint.
-    { econs 2; eauto. } all: eauto. i. des. ss.
-Qed.
+      i. econs. econs 2; eauto. } all: eauto. s. i. des.
+    exploit AThread.step_future.
+    { econs 2; eauto. } all: eauto. s. i. des.
+    econs; ss. econs.
+    i. Configuration.simplify.
+    - exploit THREADS; try apply TH1; eauto. i. des.
+      exploit AThread.rtc_tau_step_disjoint.
+      { eapply rtc_implies; try apply STEPS. eapply tau_mon.
+        i. econs. econs 2; eauto. } all: eauto. i. des.
+      exploit AThread.step_disjoint.
+      { econs 2; eauto. } all: eauto. i. des. ss.
+      symmetry. auto.
+    - exploit THREADS; try apply TH2; eauto. i. des.
+      exploit AThread.rtc_tau_step_disjoint.
+      { eapply rtc_implies; try apply STEPS. eapply tau_mon.
+        i. econs. econs 2; eauto. } all: eauto. i. des.
+      exploit AThread.step_disjoint.
+      { econs 2; eauto. } all: eauto. i. des. ss.
+    - eapply DISJOINT; [|eauto|eauto]. auto.
+    - i. Configuration.simplify.
+      exploit THREADS; try apply TH; eauto. i.
+      exploit AThread.rtc_tau_step_disjoint.
+      { eapply rtc_implies; try apply STEPS. eapply tau_mon.
+        i. econs. econs 2; eauto. } all: eauto. i. des.
+      exploit AThread.step_disjoint.
+      { econs 2; eauto. } all: eauto. i. des. ss.
+  Qed.
 
-Lemma write_no_promise mem0 loc from to val released prom1 mem1 kind
-      (WRITE: AMemory.write Memory.bot mem0 loc from to val released prom1 mem1 kind)
-  :
-    <<NOPROMISE: prom1 = Memory.bot>> /\ <<ADD: kind = Memory.op_kind_add>>.
-Proof.
-  inv WRITE. inv PROMISE.
-  - split; auto. eapply MemoryFacts.add_remove_eq; eauto.
-  - eapply Memory.split_get0 in PROMISES. des.
-    erewrite Memory.bot_get in GET0. clarify.
-  - eapply Memory.lower_get0 in PROMISES. des.
-    erewrite Memory.bot_get in GET. clarify.
-  - eapply Memory.remove_get0 in PROMISES. des.
-    erewrite Memory.bot_get in GET. clarify.
-Qed.
+  Lemma write_no_promise mem0 loc from to val released prom1 mem1 kind
+        (WRITE: AMemory.write Memory.bot mem0 loc from to val released prom1 mem1 kind)
+    :
+      <<NOPROMISE: prom1 = Memory.bot>> /\ <<ADD: kind = Memory.op_kind_add>>.
+  Proof.
+    inv WRITE. inv PROMISE.
+    - split; auto. eapply MemoryFacts.add_remove_eq; eauto.
+    - eapply Memory.split_get0 in PROMISES. des.
+      erewrite Memory.bot_get in GET0. clarify.
+    - eapply Memory.lower_get0 in PROMISES. des.
+      erewrite Memory.bot_get in GET. clarify.
+    - eapply Memory.remove_get0 in PROMISES. des.
+      erewrite Memory.bot_get in GET. clarify.
+  Qed.
 
-Lemma program_step_no_promise lang (th0 th1: Thread.t lang) e
-      (STEP: AThread.program_step e th0 th1)
-      (NOPROMISE: th0.(Thread.local).(Local.promises) = Memory.bot)
-  :
-    th1.(Thread.local).(Local.promises) = Memory.bot.
-Proof.
-  inv STEP. inv LOCAL; ss.
-  - inv LOCAL0. ss.
-  - inv LOCAL0. rewrite NOPROMISE in WRITE.
-    eapply write_no_promise in WRITE. des. auto.
-  - inv LOCAL1. inv LOCAL2. rewrite NOPROMISE in WRITE.
-    eapply write_no_promise in WRITE. des. auto.
-  - inv LOCAL0. ss.
-  - inv LOCAL0. ss.
-Qed.
+  Lemma program_step_no_promise lang (th0 th1: Thread.t lang) e
+        (STEP: AThread.program_step e th0 th1)
+        (NOPROMISE: th0.(Thread.local).(Local.promises) = Memory.bot)
+    :
+      th1.(Thread.local).(Local.promises) = Memory.bot.
+  Proof.
+    inv STEP. inv LOCAL; ss.
+    - inv LOCAL0. ss.
+    - inv LOCAL0. rewrite NOPROMISE in WRITE.
+      eapply write_no_promise in WRITE. des. auto.
+    - inv LOCAL1. inv LOCAL2. rewrite NOPROMISE in WRITE.
+      eapply write_no_promise in WRITE. des. auto.
+    - inv LOCAL0. ss.
+    - inv LOCAL0. ss.
+  Qed.
 
-Lemma program_steps_no_promise lang (th0 th1: Thread.t lang)
-      (STEP: rtc (tau (@AThread.program_step lang)) th0 th1)
-      (NOPROMISE: th0.(Thread.local).(Local.promises) = Memory.bot)
-  :
-    th1.(Thread.local).(Local.promises) = Memory.bot.
-Proof.
-  ginduction STEP; ss. i. eapply IHSTEP. inv H.
-  eapply program_step_no_promise; eauto.
-Qed.
+  Lemma program_steps_no_promise lang (th0 th1: Thread.t lang)
+        (STEP: rtc (tau (@AThread.program_step lang)) th0 th1)
+        (NOPROMISE: th0.(Thread.local).(Local.promises) = Memory.bot)
+    :
+      th1.(Thread.local).(Local.promises) = Memory.bot.
+  Proof.
+    ginduction STEP; ss. i. eapply IHSTEP. inv H.
+    eapply program_step_no_promise; eauto.
+  Qed.
 
-Lemma no_promise_spec c
-      (NOPROMISE: ~ Configuration.has_promise c)
-      tid st lc
-      (FIND: IdentMap.find tid (Configuration.threads c) = Some (st, lc))
-  :
-    lc.(Local.promises) = Memory.bot.
-Proof.
-  eapply Memory.ext. i. rewrite Memory.bot_get.
-  destruct (Memory.get loc ts (Local.promises lc)) as [[from msg]|] eqn:GET; auto.
-  exfalso. eapply NOPROMISE. econs; eauto.
-Qed.
+  Lemma no_promise_spec c
+        (NOPROMISE: ~ Configuration.has_promise c)
+        tid st lc
+        (FIND: IdentMap.find tid (Configuration.threads c) = Some (st, lc))
+    :
+      lc.(Local.promises) = Memory.bot.
+  Proof.
+    eapply Memory.ext. i. rewrite Memory.bot_get.
+    destruct (Memory.get loc ts (Local.promises lc)) as [[from msg]|] eqn:GET; auto.
+    exfalso. eapply NOPROMISE. econs; eauto.
+  Qed.
 
-Lemma configuration_step_no_promise c0 c1 tid e
-      (NOPROMISE: ~ Configuration.has_promise c0)
-      (STEP: pftstep tid e c0 c1)
-  :
-    ~ Configuration.has_promise c1.
-Proof.
-  inv STEP. ii. inv H. ss. rewrite IdentMap.gsspec in FIND. des_ifs.
-  - eapply no_promise_spec in TID; eauto.
-    eapply program_steps_no_promise in STEPS; eauto.
-    eapply program_step_no_promise in STEP0; eauto.
-    ss. rewrite STEP0 in *. rewrite Memory.bot_get in *. clarify.
-  - eapply NOPROMISE. econs; eauto.
-Qed.
+  Lemma configuration_step_no_promise c0 c1 tid e
+        (NOPROMISE: ~ Configuration.has_promise c0)
+        (STEP: step tid e c0 c1)
+    :
+      ~ Configuration.has_promise c1.
+  Proof.
+    inv STEP. ii. inv H. ss. rewrite IdentMap.gsspec in FIND. des_ifs.
+    - eapply no_promise_spec in TID; eauto.
+      eapply program_steps_no_promise in STEPS; eauto.
+      eapply program_step_no_promise in STEP0; eauto.
+      ss. rewrite STEP0 in *. rewrite Memory.bot_get in *. clarify.
+    - eapply NOPROMISE. econs; eauto.
+  Qed.
+
+End APFConfiguration.
