src/drf/APFSingle.v
@@ -31,117 +31,120 @@ Require Import APF.
 
 Set Implicit Arguments.
 
+Module APFSingle.
 
-Inductive pftstep_single: forall (e:MachineEvent.t) (tid:Ident.t) (c1 c2: Configuration.t), Prop :=
-| pftstep_single_intro
-    e tid c1 lang st1 lc1 st3 lc3 sc3 memory3
-    (TID: IdentMap.find tid c1.(Configuration.threads) = Some (existT _ lang st1, lc1))
-    (STEP: AThread.program_step e (Thread.mk _ st1 lc1 c1.(Configuration.sc) c1.(Configuration.memory)) (Thread.mk _ st3 lc3 sc3 memory3))
-    c2
-    (CONFIG: c2 = Configuration.mk (IdentMap.add tid (existT _ _ st3, lc3) c1.(Configuration.threads)) sc3 memory3)
-  :
-    pftstep_single (ThreadEvent.get_machine_event e) tid c1 c2
-.
+  Inductive step: forall (e:MachineEvent.t) (tid:Ident.t) (c1 c2: Configuration.t), Prop :=
+  | step_intro
+      e tid c1 lang st1 lc1 st3 lc3 sc3 memory3
+      (TID: IdentMap.find tid c1.(Configuration.threads) = Some (existT _ lang st1, lc1))
+      (STEP: AThread.program_step e (Thread.mk _ st1 lc1 c1.(Configuration.sc) c1.(Configuration.memory)) (Thread.mk _ st3 lc3 sc3 memory3))
+      c2
+      (CONFIG: c2 = Configuration.mk (IdentMap.add tid (existT _ _ st3, lc3) c1.(Configuration.threads)) sc3 memory3)
+    :
+      step (ThreadEvent.get_machine_event e) tid c1 c2
+  .
 
-Inductive tau_pftstep_single tid (c1 c2: Configuration.t): Prop :=
-| tau_pftstep_single_intro
-    (STEP: pftstep_single MachineEvent.silent tid c1 c2)
-.
+  Inductive tau_step tid (c1 c2: Configuration.t): Prop :=
+  | tau_step_intro
+      (STEP: step MachineEvent.silent tid c1 c2)
+  .
 
-Lemma pftstep_single_pftstep
-  :
-  pftstep_single <4= pftstep.
-Proof.
-  i. inv PR. econs; eauto.
-Qed.
+  Lemma step_long_step
+    :
+      step <4= APFConfiguration.step.
+  Proof.
+    i. inv PR. econs; eauto.
+  Qed.
 
-Lemma tau_steps_single_steps c tid lang st1 lc1 st2 lc2 sc2 mem2
-      (TID: IdentMap.find tid c.(Configuration.threads) = Some (existT _ lang st1, lc1))
-      (STEPS: Relation_Operators.clos_refl_trans_n1 _ (tau (@AThread.program_step _)) (Thread.mk _ st1 lc1 c.(Configuration.sc) c.(Configuration.memory)) (Thread.mk _ st2 lc2 sc2 mem2))
-  :
-    exists ths',
-      (<<STEPS: Relation_Operators.clos_refl_trans_n1 _ (tau_pftstep_single tid) c (Configuration.mk ths' sc2 mem2)>>) /\
-      ((ths' = IdentMap.add tid (existT _ lang st2, lc2) c.(Configuration.threads)) \/
-       (ths' = c.(Configuration.threads) /\ st1 = st2 /\ lc1 = lc2)).
-Proof.
-  remember (Thread.mk _ st1 lc1 (Configuration.sc c) (Configuration.memory c)) as th1.
-  remember (Thread.mk _ st2 lc2 sc2 mem2) as th2. ginduction STEPS.
-  - i. clarify. destruct c. esplits.
-    + ss. econs 1.
-    + ss. right. auto.
-  - i. clarify. destruct y. inv H. exploit IHSTEPS; eauto. i. des; clarify.
-    + destruct c. ss. esplits.
-      * econs 2; eauto. econs; eauto. rewrite <- EVENT. econs; eauto.
-        ss. rewrite IdentMap.gss. ss.
-      * ss. left. eapply IdentMap.add_add_eq.
-    + destruct c. ss. esplits.
-      * econs 2; eauto. econs; eauto. rewrite <- EVENT. econs; eauto.
-      * ss. left. auto.
-Qed.
+  Lemma tau_steps_single_steps c tid lang st1 lc1 st2 lc2 sc2 mem2
+        (TID: IdentMap.find tid c.(Configuration.threads) = Some (existT _ lang st1, lc1))
+        (STEPS: Relation_Operators.clos_refl_trans_n1 _ (tau (@AThread.program_step _)) (Thread.mk _ st1 lc1 c.(Configuration.sc) c.(Configuration.memory)) (Thread.mk _ st2 lc2 sc2 mem2))
+    :
+      exists ths',
+        (<<STEPS: Relation_Operators.clos_refl_trans_n1 _ (tau_step tid) c (Configuration.mk ths' sc2 mem2)>>) /\
+        ((ths' = IdentMap.add tid (existT _ lang st2, lc2) c.(Configuration.threads)) \/
+         (ths' = c.(Configuration.threads) /\ st1 = st2 /\ lc1 = lc2)).
+  Proof.
+    remember (Thread.mk _ st1 lc1 (Configuration.sc c) (Configuration.memory c)) as th1.
+    remember (Thread.mk _ st2 lc2 sc2 mem2) as th2. ginduction STEPS.
+    - i. clarify. destruct c. esplits.
+      + ss. econs 1.
+      + ss. right. auto.
+    - i. clarify. destruct y. inv H. exploit IHSTEPS; eauto. i. des; clarify.
+      + destruct c. ss. esplits.
+        * econs 2; eauto. econs; eauto. rewrite <- EVENT. econs; eauto.
+          ss. rewrite IdentMap.gss. ss.
+        * ss. left. eapply IdentMap.add_add_eq.
+      + destruct c. ss. esplits.
+        * econs 2; eauto. econs; eauto. rewrite <- EVENT. econs; eauto.
+        * ss. left. auto.
+  Qed.
 
-Lemma pftstep_single_sim c0 c1 e tid
-      (STEP: pftstep e tid c0 c1)
-  :
-    exists c',
-      (<<STEPS: rtc (tau_pftstep_single tid) c0 c'>>) /\
-      (<<STEP: pftstep_single e tid c' c1>>).
-Proof.
-  inv STEP.
-  eapply Operators_Properties.clos_rt1n_rt in STEPS.
-  eapply Operators_Properties.clos_rt_rtn1 in STEPS.
-  destruct e2. exploit tau_steps_single_steps; eauto. i. des; clarify.
-  - eapply Operators_Properties.clos_rtn1_rt in STEPS0.
-    eapply Operators_Properties.clos_rt_rt1n in STEPS0.
-    esplits; eauto. econs.
-    + ss. rewrite IdentMap.gss. ss.
-    + ss. eauto.
-    + ss. f_equal. symmetry. eapply IdentMap.add_add_eq.
-  - eapply Operators_Properties.clos_rtn1_rt in STEPS0.
-    eapply Operators_Properties.clos_rt_rt1n in STEPS0.
-    esplits; eauto. econs; eauto.
-Qed.
+  Lemma step_sim c0 c1 e tid
+        (STEP: APFConfiguration.step e tid c0 c1)
+    :
+      exists c',
+        (<<STEPS: rtc (tau_step tid) c0 c'>>) /\
+        (<<STEP: step e tid c' c1>>).
+  Proof.
+    inv STEP.
+    eapply Operators_Properties.clos_rt1n_rt in STEPS.
+    eapply Operators_Properties.clos_rt_rtn1 in STEPS.
+    destruct e2. exploit tau_steps_single_steps; eauto. i. des; clarify.
+    - eapply Operators_Properties.clos_rtn1_rt in STEPS0.
+      eapply Operators_Properties.clos_rt_rt1n in STEPS0.
+      esplits; eauto. econs.
+      + ss. rewrite IdentMap.gss. ss.
+      + ss. eauto.
+      + ss. f_equal. symmetry. eapply IdentMap.add_add_eq.
+    - eapply Operators_Properties.clos_rtn1_rt in STEPS0.
+      eapply Operators_Properties.clos_rt_rt1n in STEPS0.
+      esplits; eauto. econs; eauto.
+  Qed.
 
-Lemma taus_pftstep_single tid c0 c1 beh
-      (TAUS: rtc (tau_pftstep_single tid) c0 c1)
-      (BEH: behaviors pftstep_single c1 beh)
-  :
-    behaviors pftstep_single c0 beh.
-Proof.
-  ginduction TAUS; i; auto.
-  eapply IHTAUS in BEH. inv H. econs 4; eauto.
-Qed.
+  Lemma taus_step tid c0 c1 beh
+        (TAUS: rtc (tau_step tid) c0 c1)
+        (BEH: behaviors step c1 beh)
+    :
+      behaviors step c0 beh.
+  Proof.
+    ginduction TAUS; i; auto.
+    eapply IHTAUS in BEH. inv H. econs 4; eauto.
+  Qed.
 
-Lemma pftstep_equiv c
-  :
-    behaviors pftstep c
-    <1=
-    behaviors pftstep_single c.
-Proof.
-  ii. ginduction PR.
-  - econs; ss.
-  - exploit pftstep_single_sim; eauto. i. des.
-    eapply taus_pftstep_single in STEPS; eauto. econs 2; eauto.
-  - exploit pftstep_single_sim; eauto. i. des.
-    eapply taus_pftstep_single in STEPS; eauto. econs 3; eauto.
-  - exploit pftstep_single_sim; eauto. i. des.
-    eapply taus_pftstep_single in STEPS; eauto. econs 4; eauto.
-Qed.
+  Lemma long_step_equiv c
+    :
+      behaviors APFConfiguration.step c
+      <1=
+      behaviors step c.
+  Proof.
+    ii. ginduction PR.
+    - econs; ss.
+    - exploit step_sim; eauto. i. des.
+      eapply taus_step in STEPS; eauto. econs 2; eauto.
+    - exploit step_sim; eauto. i. des.
+      eapply taus_step in STEPS; eauto. econs 3; eauto.
+    - exploit step_sim; eauto. i. des.
+      eapply taus_step in STEPS; eauto. econs 4; eauto.
+  Qed.
 
-Lemma pftstep_equiv2 c
-  :
-    behaviors pftstep_single c
-    <1=
-    behaviors pftstep c.
-Proof.
-  eapply le_step_behavior_improve; eauto.
-  eapply pftstep_single_pftstep.
-Qed.
+  Lemma long_step_equiv2 c
+    :
+      behaviors step c
+      <1=
+      behaviors APFConfiguration.step c.
+  Proof.
+    eapply le_step_behavior_improve; eauto.
+    eapply step_long_step.
+  Qed.
 
-Definition pftstep_single_all (c0 c1: Configuration.t) :=
-  union (fun e => union (pftstep_single e)) c0 c1.
-Hint Unfold pftstep_single_all.
+  Definition step_all (c0 c1: Configuration.t) :=
+    union (fun e => union (step e)) c0 c1.
+  Hint Unfold step_all.
 
-Definition pf_racefree (c1:Configuration.t): Prop :=
-  forall c2
-         (STEPS: rtc pftstep_single_all c1 c2)
-         (RACE: pf_race c2), False.
+  Definition pf_racefree (c1:Configuration.t): Prop :=
+    forall c2
+           (STEPS: rtc step_all c1 c2)
+           (RACE: pf_race c2), False.
+
+End APFSingle.
